Guarded2Network/Lemmas.lean
@@ -12,6 +12,7 @@ public import Guarded2Network.Lemmas.Reorder
 public import Guarded2Network.Lemmas.Precondition
 public import Guarded2Network.Lemmas.AtomicBranch
 public import Guarded2Network.Lemmas.AtomicBlock
+public import Guarded2Network.Lemmas.Thread
 public import Guarded2Network.Lemmas.Process
 public import Guarded2Network.Lemmas.Algorithm
 public import Core.NetworkPlusCal.Semantics.Lemmas
